\section{Derivadas simples}
	\begin{table}[H]
		\caption{Derivadas simples}
		\label{derivadas_simples}
		\centering
		%\ABNTEXfontereduzida		
		\begin{tabular}{|lclclcl|}
			$y$ & $=$ & $c$            & $\Rightarrow$ & $y'$ & $=$ & $0$                       \\
			$y$ & $=$ & $x$            & $\Rightarrow$ & $y'$ & $=$ & $1$                       \\
			$y$ & $=$ & $x^c$          & $\Rightarrow$ & $y'$ & $=$ & $cx^{c - 1}$              \\
			$y$ & $=$ & $\e^x$         & $\Rightarrow$ & $y'$ & $=$ & $\e^x$                    \\
			$y$ & $=$ & $\ln |x|$      & $\Rightarrow$ & $y'$ & $=$ & $\dfrac{1}{x}$            \\
			$y$ & $=$ & $uv$           & $\Rightarrow$ & $y'$ & $=$ & $u'v + uv'$               \\
			$y$ & $=$ & $\dfrac{u}{v}$ & $\Rightarrow$ & $y'$ & $=$ & $\dfrac{u'v - uv'}{v^2}$  \\
			$y$ & $=$ & $u^c$          & $\Rightarrow$ & $y'$ & $=$ & $cu^{c - 1}u'$            \\
			$y$ & $=$ & $\e^u$         & $\Rightarrow$ & $y'$ & $=$ & $\e^uu'$                  \\
			$y$ & $=$ & $c^u$          & $\Rightarrow$ & $y'$ & $=$ & $c^uu'ln|c|$              \\
			$y$ & $=$ & $\ln |u|$      & $\Rightarrow$ & $y'$ & $=$ & $\dfrac{u'}{u}$           \\
			$y$ & $=$ & $\log_c|u|$    & $\Rightarrow$ & $y'$ & $=$ & $\dfrac{u'}{u}\log_c|\e|$
		\end{tabular}		
	\end{table}

\section{Derivadas trigonométricas}
	\begin{table}[H]
		\caption{Derivadas trigonométricas}
		\label{derivadas_trigometricas}
		\centering
		%\ABNTEXfontereduzida		
		\begin{tabular}{|lclclcl|}
			$y$ & $=$ & $\sen(x)$       & $\Rightarrow$ & $y'$ & $=$ & $\cos(x)$                       \\
			$y$ & $=$ & $\cos(x)$       & $\Rightarrow$ & $y'$ & $=$ & $-\sen(x)$                      \\
			$y$ & $=$ & $\tg(x)$        & $\Rightarrow$ & $y'$ & $=$ & $\sec^2(x)$                     \\
			$y$ & $=$ & $\cotg(x)$      & $\Rightarrow$ & $y'$ & $=$ & $-\cossec^2(x)$                 \\
			$y$ & $=$ & $\sec(x)$       & $\Rightarrow$ & $y'$ & $=$ & $\sec(x)\tg(x)$                 \\
			$y$ & $=$ & $\cossec(x)$    & $\Rightarrow$ & $y'$ & $=$ & $-\cossec(x)\cotg(x)$           \\
			$y$ & $=$ & $\arcsen(x)$    & $\Rightarrow$ & $y'$ & $=$ & $\dfrac{1}{\sqrt{1 - x^2}}$     \\
			$y$ & $=$ & $\arccos(x)$    & $\Rightarrow$ & $y'$ & $=$ & $\dfrac{-1}{\sqrt{1 - x^2}}$    \\
			$y$ & $=$ & $\arctg(x)$     & $\Rightarrow$ & $y'$ & $=$ & $\dfrac{1}{1 + x^2}$            \\
			$y$ & $=$ & $\arccotg(x)$   & $\Rightarrow$ & $y'$ & $=$ & $\dfrac{-1}{1 + x^2}$           \\
			$y$ & $=$ & $\arcsec(x)$    & $\Rightarrow$ & $y'$ & $=$ & $\dfrac{1}{|x|\sqrt{x^2 - 1}}$  \\
			$y$ & $=$ & $\arccossec(x)$ & $\Rightarrow$ & $y'$ & $=$ & $\dfrac{-1}{|x|\sqrt{x^2 - 1}}$
		\end{tabular}		
	\end{table}