\begin{enumerate}
	\item Exerc√≠cio
	
	\begin{equation*}
		\iiint_R \e^{\sqrt{\left(x^2 + y^2 + z^2\right)^3}}\, dv
	\end{equation*}
	\begin{equation*}
		R = \{(x,y,z) \,|\, x^2 + y^2 + z^2 \leq 1\}
	\end{equation*}
	
	\begin{equation*}
		x^2 + y^2 + z^2 = r^2 \Rightarrow \e^{\sqrt{\left(x^2 + y^2 + z^2\right)^3}} = \e^{\sqrt{\left(r^2\right)^3}} = \e^{r^3}
	\end{equation*}
	\begin{equation*}
		dv = dxdydz = r^2\sen(\varphi)\, dr d\theta d\varphi
	\end{equation*}
	\begin{equation*}
		x^2 + y^2 + z^2 = r^2 = 1^2 = 1
	\end{equation*}
	\begin{equation*}
		0 \leq r \leq 1,\, 0 \leq \theta \leq 2\pi,\, 0 \leq \varphi \leq \pi
	\end{equation*}
	\begin{align*}
		\int_0^1 \int_0^{2\pi} \int_0^{\pi} e^{r^3} r^2\sen(\varphi)\, d\varphi d\theta dr = \int_0^1 e^{r^3} r^2\,dr \int_0^{2\pi} d\theta \int_0^{\pi} \sen(\varphi)\, d\varphi =\\ \int_0^1 e^u \dfrac{du}{3} \left[\theta\right]_0^{2\pi} \left[-\cos(\varphi)\right]_0^{\pi} = \dfrac{1}{3} \left[e^{r^3}\right]_0^1 2\pi \left(-\cos(\pi) + \cos(0)\right) = \dfrac{2\pi}{3} \left(e^{1^3} - e^{0^3}\right)(1+1) =\\ \dfrac{4\pi}{3} (e - 1)
	\end{align*}
	\begin{equation*}
		u = r^3 \Rightarrow \dfrac{du}{3} = r^2\, dr
	\end{equation*}
\end{enumerate}