\begin{enumerate}
	\item Exercício
	
	Calcule a integral tripla abaixo.
	
	\begin{equation*}
		\iiint_R 12xy^2z^3\,dv
	\end{equation*}
	\begin{equation*}
		R = \left\{(x, y, z) \in \mathbb{R}^3 \,|\, -1 \leq x \leq 2,\, 0 \leq y \leq 3,\, 0 \leq z \leq 2\right\}
	\end{equation*}
	
	\begin{equation*}
		dv = dxdydz
	\end{equation*}
	\begin{gather*}
		\iiint_R 12xy^2z^3\,dv = \int_{-1}^2 \int_0^3 \int_0^2 12xy^2z^3\, dz dy dx = 12\int_{-1}^2 x\, dx \int_0^3 y^2\, dy \int_0^2 z^3\, dz =\\ {\overstrike{12}}\left[\dfrac{x^2}{2}\right]_{-1}^2 \left[\dfrac{y^3}{\overstrike{3}}\right]_0^3 \left[\dfrac{z^4}{\overstrike{4}}\right]_0^2 = \dfrac{1}{2}\left[x^2\right]_{-1}^2 \left[y^3\right]_0^3 \left[z^4\right]_0^2 = \dfrac{1}{2}\left(2^2 - (-1)^2\right)3^3 2^4 = \dfrac{1}{2}3\cdot27\cdot16 = 648
	\end{gather*}
	
	\item Exercício
	
	Observe a integral e preencha os retângulos abaixo.
	
	\begin{equation*}
		\int_1^5 \int_2^4 \int_3^6 f(x,y,z)\, dxdzdy	
	\end{equation*}
	\begin{equation*}
		[3] \leq x \leq [6]
	\end{equation*}
	\begin{equation*}
		[1] \leq y \leq [5]
	\end{equation*}
	\begin{equation*}
		[2] \leq z \leq [4]
	\end{equation*}
	
	\item Exercício
	
	\begin{gather*}
		\int_{-1}^1 \int_0^2 \int_0^1 \left(x^2 + y^2 + z^2\right)\, dxdydz = \int_{-1}^1 dz \int_0^2 dy \int_0^1 \left(x^2 + y^2 + z^2\right)\, dx =\\ \int_{-1}^1 dz \int_0^2 dy\left( \int_0^1 x^2\, dx + y^2\int_0^1 dx + z^2\int_0^1 dx\right) =\\ \int_{-1}^1 dz \int_0^2 dy \int_0^1 x^2\, dx + \int_{-1}^1 dz \int_0^2 y^2\, dy \int_0^1 dx + \int_{-1}^1 z^2\, dz \int_0^2 dy \int_0^1 dx =\\ [z]_{-1}^1 [y]_0^2 \left[\dfrac{x^3}{3}\right]_0^1 + [z]_{-1}^1 \left[\dfrac{y^3}{3}\right]_0^2 [x]_0^1 + \left[\dfrac{z^3}{3}\right]_{-1}^1 [y]_0^2 [x]_0^1 =\\ [z]_{-1}^1 [y]_0^2 \dfrac{1}{3}\left[x^3\right]_0^1 + [z]_{-1}^1 \dfrac{1}{3}\left[y^3\right]_0^2 [x]_0^1 + \dfrac{1}{3}\left[z^3\right]_{-1}^1 [y]_0^2 [x]_0^1 =\\ \dfrac{1}{3}\left([1 + 1]2\cdot1^3 + [1 + 1]2^3\cdot1 + \left[1^3 - (-1)^3\right]2\cdot1\right) = \dfrac{1}{3}\left(4 + 16 + 4\right) = \dfrac{24}{3} = 8
	\end{gather*}
	
	\item Exercício
	
	\begin{gather*}
		\int_0^2 \int_{-1}^{y^2} \int_{-1}^z yz\, dxdzdy = \int_0^2 \int_{-1}^{y^2}\left(yz\int_{-1}^z dx\right)\, dzdy = \int_0^2 \int_{-1}^{y^2} [yzx]_{-1}^z\, dzdy =\\ \int_0^2 \int_{-1}^{y^2} [yz^2 + yz]\, dzdy = \int_0^2\left(y\int_{-1}^{y^2} z^2\, dz + y\int_{-1}^{y^2} z\, dz\right)\, dy = \int_0^2 \left[y\dfrac{z^3}{3} + y\dfrac{z^2}{2}\right]_{-1}^{y^2}\, dy =\\ \int_0^2 \left[\dfrac{2yz^3 + 3yz^2}{6}\right]_{-1}^{y^2}\, dy = \dfrac{1}{6} \int_0^2 \left[yz^2\left(2z + 3\right)\right]_{-1}^{y^2}\, dy =\\ \dfrac{1}{6} \int_0^2 \left[y\left(y^2\right)^2\left(2y^2 + 3\right) - y(-1)^2\left(2(-1) + 3\right)\right]\, dy = \dfrac{1}{6} \int_0^2 \left[y^5\left(2y^2 + 3\right) - y\right]\, dy =\\ \dfrac{1}{6} \int_0^2 \left(2y^7 + 3y^5 - y\right)\, dy = \dfrac{1}{6} \left[\dfrac{2y^8}{8} + \dfrac{3y^6}{6} - \dfrac{y^2}{2}\right]_0^2 = \dfrac{1}{6} \left[\dfrac{y^8}{4} + \dfrac{y^6}{2} - \dfrac{y^2}{2}\right]_0^2 =\\ \dfrac{1}{6} \left[\dfrac{y^8 + 2y^6 - 2y^2}{4}\right]_0^2 = \dfrac{1}{24}\left[y^2\left(y^6 + 2y^4 - 2\right)\right]_0^2 = \dfrac{1}{24}\left[2^2\left(2^6 + 2\cdot2^4 - 2\right)\right] =\\ \dfrac{1}{24} \left[4\left(64 + 32 - 2\right)\right] = \dfrac{94}{6} = \dfrac{47}{3}
	\end{gather*}
\end{enumerate}